Model probabilistic partial functions explicitly

src/Distributions/Bernoulli/Model.dfy
@@ -6,15 +6,16 @@
 module Bernoulli.Model {
   import Uniform
   import Monad
+  import Partial
 
   // Footnote 5, p. 82
-  function Sample(numer: nat, denom: nat): (f: Monad.Hurd<bool>)
+  ghost function Sample(numer: nat, denom: nat): (f: Partial.Hurd<bool>)
     requires denom != 0
     requires numer <= denom
-    ensures forall s :: f(s).0 == (Uniform.Model.Sample(denom)(s).0 < numer)
+    ensures forall s :: f(s).0 == Uniform.Model.Sample(denom)(s).0.Map(x => x < numer)
     ensures forall s :: f(s).1 == Uniform.Model.Sample(denom)(s).1
   {
-    Monad.Bind(Uniform.Model.Sample(denom), (k: nat) => Monad.Return(k < numer))
+    Partial.Map((k: nat) => k < numer, Uniform.Model.Sample(denom))
   }
 
 }
