src/Distributions/BernoulliExpNeg/Model.dfy
@@ -7,70 +7,71 @@ module BernoulliExpNeg.Model {
   import Rationals
   import Uniform
   import Monad
+  import Partial
   import WhileAndUntil
   import BernoulliModel = Bernoulli.Model
 
-  function Sample(gamma: Rationals.Rational): Monad.Hurd<bool>
+  ghost function Sample(gamma: Rationals.Rational): Partial.Hurd<bool>
     requires gamma.denom != 0
     requires gamma.numer >= 0
   {
-    Monad.Bind(
-      GammaReductionLoop(gamma),
+    Partial.Bind(
+      GammaReductionLoop(true, gamma),
       (bgamma: (bool, Rationals.Rational)) =>
         if bgamma.0 then
           SampleGammaLe1(bgamma.1)
         else
-          Monad.Return(false)
+          Partial.Return(false)
     )
   }
 
-  function GammaReductionLoop(gamma: Rationals.Rational): Monad.Hurd<(bool, Rationals.Rational)>
+  ghost function GammaReductionLoop(b: bool, gamma: Rationals.Rational): Partial.Hurd<(bool, Rationals.Rational)>
     requires gamma.numer >= 0
+    decreases gamma.numer
   {
-    assume {:axiom} false; // assume termination
-    WhileAndUntil.ProbWhile(
-      (bgamma: (bool, Rationals.Rational)) => bgamma.0 && bgamma.1.denom <= bgamma.1.numer,
-      GammaReductionLoopIter,
-      (true, gamma)
-    )
+    if b && gamma.denom <= gamma.numer
+    then
+      Partial.Bind(
+        SampleGammaLe1(Rationals.Int(1)),
+        b' => GammaReductionLoop(b', Rationals.Rational(gamma.numer - gamma.denom, gamma.denom))
+      )
+    else
+      Partial.Return((b, gamma))
   }
 
-  function GammaReductionLoopIter(bgamma: (bool, Rationals.Rational)): Monad.Hurd<(bool, Rationals.Rational)>
-    requires bgamma.1.numer >= 0
-  {
-    Monad.Bind(
-      SampleGammaLe1(Rationals.Int(1)),
-      b' => Monad.Return((b', Rationals.Rational(bgamma.1.numer - bgamma.1.denom, bgamma.1.denom)))
-    )
-  }
-
-  function SampleGammaLe1(gamma: Rationals.Rational): Monad.Hurd<bool>
+  ghost function SampleGammaLe1(gamma: Rationals.Rational): Partial.Hurd<bool>
   {
     if 0 <= gamma.numer <= gamma.denom
-    then Monad.Bind(
+    then Partial.Bind(
            GammaLe1Loop(gamma, (true, 0)),
-           (ak: (bool, nat)) => Monad.Return(ak.1 % 2 == 1)
+           (ak: (bool, nat)) => Partial.Return(ak.1 % 2 == 1)
          )
-    else Monad.Return(false) // to keep this function total, we return a dummy value here
+    else Partial.Return(false) // to keep this function total, we return a dummy value here
   }
 
-  function GammaLe1Loop(gamma: Rationals.Rational, ak: (bool, nat)): Monad.Hurd<(bool, nat)>
+  ghost function GammaLe1Loop(gamma: Rationals.Rational, ak: (bool, nat)): Partial.Hurd<(bool, nat)>
     requires 0 <= gamma.numer <= gamma.denom
   {
     assume {:axiom} false; // assume termination
-    WhileAndUntil.ProbWhile(
-      (ak: (bool, nat)) => ak.0,
-      (ak: (bool, nat)) => GammaLe1LoopIter(gamma, ak),
-      ak
+    Partial.Bind(
+      WhileAndUntil.ProbWhile(
+        (ak: Partial.Wrap<(bool, nat)>) => ak.Satisfies((x: (bool, nat)) => x.0),
+        (ak: Partial.Wrap<(bool, nat)>) =>
+          match ak
+          case Terminating(ak) => GammaLe1LoopIter(gamma, ak)
+          case Diverging => Partial.Diverge(),
+        Partial.Terminating(ak)
+      ),
+      (ak: Partial.Wrap<(bool, nat)>) => Monad.Return(ak)
     )
   }
 
-  function GammaLe1LoopIter(gamma: Rationals.Rational, ak: (bool, nat)): Monad.Hurd<(bool, nat)>
+  ghost function GammaLe1LoopIter(gamma: Rationals.Rational, ak: (bool, nat)): Partial.Hurd<(bool, nat)>
     requires 0 <= gamma.numer <= gamma.denom
   {
-    Monad.Bind(
+    Partial.Bind(
       BernoulliModel.Sample(gamma.numer, (ak.1 + 1) * gamma.denom),
-      (a': bool) => Monad.Return((a', ak.1 + 1))
+      (a': bool) => Partial.Return((a', ak.1 + 1))
     )
   }
 }
