src/Distributions/Bernoulli/Correctness.dfy
@@ -10,6 +10,7 @@ module Bernoulli.Correctness {
   import RandomNumberGenerator
   import Independence
   import Monad
+  import Partial
   import Model
 
   /*******
@@ -22,7 +23,7 @@ module Bernoulli.Correctness {
     ensures Independence.IsIndepFn(Model.Sample(m, n))
   {
     var f := Uniform.Model.Sample(n);
-    var g := (k: nat) => Monad.Return(k < m);
+    var g := (k: nat) => Partial.Return(k < m);
 
     assert Independence.IsIndepFn(f) by {
       Uniform.Correctness.SampleIsIndepFn(n);
@@ -34,7 +35,7 @@ module Bernoulli.Correctness {
       }
     }
 
-    Independence.IndepFnIsCompositional(f, g);
+    Independence.IndepFnIsCompositionalPartial(f, g);
   }
 
 
@@ -42,18 +43,18 @@ module Bernoulli.Correctness {
     requires n != 0
     requires m <= n
     ensures
-      var e := iset s | Model.Sample(m, n)(s).0;
+      var e := iset s | Model.Sample(m, n)(s).0 == Partial.Terminating(true);
       && e in RandomNumberGenerator.event_space
       && RandomNumberGenerator.mu(e) == m as real / n as real
   {
-    var e := iset s | Model.Sample(m, n)(s).0;
+    var e := iset s | Model.Sample(m, n)(s).0 == Partial.Terminating(true);
 
     if m == 0 {
       assert e == iset{} by {
-        forall s ensures !Model.Sample(m, n)(s).0 {
+        forall s ensures Model.Sample(m, n)(s).0 == Partial.Terminating(false) {
           calc {
-            Model.Sample(m, n)(s).0;
-            Uniform.Model.Sample(n)(s).0 < 0;
+            Model.Sample(m, n)(s).0.value;
+            Uniform.Model.Sample(n)(s).0.value < 0;
             false;
           }
         }
@@ -65,22 +66,22 @@ module Bernoulli.Correctness {
         assert MeasureTheory.IsPositive(RandomNumberGenerator.event_space, RandomNumberGenerator.mu);
       }
     } else {
-      var e1 := iset s | Uniform.Model.Sample(n)(s).0 == m-1;
-      var e2 := (iset s {:trigger Uniform.Model.Sample(n)(s).0} | Model.Sample(m-1, n)(s).0);
+      var e1 := iset s | Uniform.Model.Sample(n)(s).0 == Partial.Terminating(m-1);
+      var e2 := (iset s {:trigger Uniform.Model.Sample(n)(s).0} | Model.Sample(m-1, n)(s).0 == Partial.Terminating(true));
 
-      assert (iset s | Uniform.Model.Sample(n)(s).0 < m-1) == e2 by {
-        assert (iset s | Uniform.Model.Sample(n)(s).0 < m-1) == (iset s {:trigger Uniform.Model.Sample(n)(s).0} | Model.Sample(m-1, n)(s).0) by {
-          forall s ensures Uniform.Model.Sample(n)(s).0 < m-1 <==> Model.Sample(m-1, n)(s).0 {
-            assert Uniform.Model.Sample(n)(s).0 < m-1 <==> Model.Sample(m-1, n)(s).0;
+      assert (iset s | Uniform.Model.Sample(n)(s).0.Satisfies(x => x < m-1)) == e2 by {
+        assert (iset s | Uniform.Model.Sample(n)(s).0.Satisfies(x => x < m-1)) == (iset s {:trigger Uniform.Model.Sample(n)(s).0} | Model.Sample(m-1, n)(s).0 == Partial.Terminating(true)) by {
+          forall s ensures Uniform.Model.Sample(n)(s).0.Satisfies(x => x < m-1) <==> Model.Sample(m-1, n)(s).0.Satisfies(x => x) {
+            assert Uniform.Model.Sample(n)(s).0.Satisfies(x => x < m-1) <==> Model.Sample(m-1, n)(s).0.Satisfies(x => x);
           }
         }
       }
 
       calc {
         e;
-        iset s | Uniform.Model.Sample(n)(s).0 < m;
-        iset s | Uniform.Model.Sample(n)(s).0 == m-1 || Uniform.Model.Sample(n)(s).0 < m-1;
-        (iset s | Uniform.Model.Sample(n)(s).0 == m-1) + (iset s | Uniform.Model.Sample(n)(s).0 < m-1);
+        iset s | Uniform.Model.Sample(n)(s).0.Satisfies(x => x < m);
+        iset s | Uniform.Model.Sample(n)(s).0.Satisfies(x => x == m-1) || Uniform.Model.Sample(n)(s).0.Satisfies(x => x < m-1);
+        (iset s | Uniform.Model.Sample(n)(s).0.Satisfies(x => x == m-1)) + (iset s | Uniform.Model.Sample(n)(s).0.Satisfies(x => x < m-1));
         e1 + e2;
       }
 
