src/Distributions/BernoulliExpNeg/Correctness.dfy
@@ -7,12 +7,13 @@ module BernoulliExpNeg.Correctness {
   import Rationals
   import Exponential
   import RandomNumberGenerator
+  import Partial
   import Independence
   import Model
 
   lemma {:axiom} Correctness(gamma: Rationals.Rational)
     requires 0 <= gamma.numer
-    ensures RandomNumberGenerator.mu(iset s | Model.Sample(gamma)(s).0) == Exponential.Exp(-Rationals.ToReal(gamma))
+    ensures RandomNumberGenerator.mu(iset s | Model.Sample(gamma)(s).0 == Partial.Terminating(true)) == Exponential.Exp(-Rationals.ToReal(gamma))
 
   lemma {:axiom} SampleIsIndepFn(gamma: Rationals.Rational)
     requires 0 <= gamma.numer
