src/Distributions/Uniform/Interface.dfy
@@ -6,6 +6,7 @@
 module Uniform.Interface {
   import Coin
   import Model
+  import Partial
   import UniformPowerOfTwo
 
   trait {:termination false} Trait extends Coin.Interface.Trait, UniformPowerOfTwo.Interface.Trait {
@@ -15,18 +16,18 @@ module Uniform.Interface {
       decreases *
       requires n > 0
       ensures u < n
-      ensures Model.Sample(n)(old(s)) == (u, s)
+      ensures Model.Sample(n)(old(s)) == (Partial.Terminating(u), s)
 
     method UniformIntervalSample(a: int, b: int) returns (u: int)
       modifies this
       decreases *
       requires a < b
       ensures a <= u < b
-      ensures Model.IntervalSample(a, b)(old(s)) == (u, s)
+      ensures Model.IntervalSample(a, b)(old(s)) == (Partial.Terminating(u), s)
     {
       var v := UniformSample(b - a);
-      assert Model.Sample(b-a)(old(s)) == (v, s);
-      assert Model.IntervalSample(a, b)(old(s)) == (a + v, s);
+      assert Model.Sample(b-a)(old(s)) == (Partial.Terminating(v), s);
+      assert Model.IntervalSample(a, b)(old(s)) == (Partial.Terminating(a + v), s);
       u := a + v;
     }
 
