src/ProbabilisticProgramming/PartialMonad.dfy
@@ -1,0 +1,130 @@
+/*******************************************************************************
+ *  Copyright by the contributors to the Dafny Project
+ *  SPDX-License-Identifier: MIT
+ *******************************************************************************/
+
+module Partial {
+  import Monad
+  import RandomNumberGenerator
+  import MeasureTheory
+
+  /************
+   Definitions
+  ************/
+
+  datatype Wrap<T> = Diverging | Terminating(value: T) {
+    predicate IsFailure() {
+      Diverging?
+    }
+
+    function PropagateFailure(): Wrap<T> {
+      Diverging
+    }
+
+    function Extract(): T
+      requires !IsFailure()
+    {
+      this.value
+    }
+
+    function Map<U>(f: T -> U): Wrap<U> {
+      match this
+      case Terminating(value) => Terminating(f(value))
+      case Diverging => Diverging
+    }
+
+    function UnwrapOr(default: T): T {
+      match this
+      case Terminating(value) => value
+      case Diverging => default
+    }
+
+    function Satisfies(f: T -> bool): bool {
+      this.Map(f).UnwrapOr(false)
+    }
+
+    function Bind<U>(f: T -> Wrap<U>): Wrap<U> {
+      match this
+      case Terminating(value) => f(value)
+      case Diverging => Diverging
+    }
+  }
+
+  type Hurd<A> = RandomNumberGenerator.RNG -> (Wrap<A>, RandomNumberGenerator.RNG)
+
+  // Equation (3.4)
+  function Bind<A,B>(f: Hurd<A>, g: A -> Hurd<B>): Hurd<B> {
+    (s: RandomNumberGenerator.RNG) =>
+      var (a, s') := f(s);
+      match a
+      case Terminating(a) => g(a)(s')
+      case Diverging => (Diverging, s')
+  }
+
+  function Composition<A,B,C>(f: A -> Hurd<B>, g: B -> Hurd<C>): A -> Hurd<C> {
+    (a: A) => Bind(f(a), g)
+  }
+
+  function Diverge<A>(): Hurd<A> {
+    Monad.Return(Diverging)
+  }
+
+  function Return<A>(a: A): Hurd<A> {
+    Monad.Return(Terminating(a))
+  }
+
+  function Flatten<A>(f: Hurd<Wrap<A>>): Hurd<A> {
+    Bind(f, (a: Wrap<A>) =>
+      match a
+      case Terminating(a) => Return(a)
+      case Diverging => Diverge())
+  }
+
+  function Map<A,B>(f: A -> B, m: Hurd<A>): Hurd<B> {
+    Bind(m, (a: A) => Return(f(a)))
+  }
+
+  function Join<A>(ff: Hurd<Hurd<A>>): Hurd<A> {
+    Bind(ff, a => a)
+  }
+
+  /*******
+   Lemmas
+  *******/
+
+  lemma UnitalityBindReturn<A,B>(a: A, g: A -> Hurd<B>, s: RandomNumberGenerator.RNG)
+    ensures Bind(Return(a), g)(s) == g(a)(s)
+  {}
+
+  lemma BindIsAssociative<A,B,C>(f: Hurd<A>, g: A -> Hurd<B>, h: B -> Hurd<C>, s: RandomNumberGenerator.RNG)
+    ensures Bind(Bind(f, g), h)(s) == Bind(f, (a: A) => Bind(g(a), h))(s)
+  {
+    assume {:axiom} false; // todo
+  }
+
+  lemma CompositionIsAssociative<A,B,C,D>(f: A -> Hurd<B>, g: B -> Hurd<C>, h: C -> Hurd<D>, a: A, s: RandomNumberGenerator.RNG)
+    ensures Composition(Composition(f, g), h)(a)(s) == Composition(f, Composition(g, h))(a)(s)
+  {
+    BindIsAssociative(f(a), g, h, s);
+  }
+
+  lemma UnitalityJoinReturn<A>(f: Hurd<A>, s: RandomNumberGenerator.RNG)
+    ensures Join(Map(Return, f))(s) == Join(Return(f))(s)
+  {
+    var (a, t) := f(s);
+    calc {
+      Join(Return(f))(s);
+    ==
+      (a, t);
+    ==
+      Join(Map(Return, f))(s);
+    }
+  }
+
+  lemma JoinIsAssociative<A>(fff: Hurd<Hurd<Hurd<A>>>, s: RandomNumberGenerator.RNG)
+    ensures Join(Map(Join, fff))(s) == Join(Join(fff))(s)
+  {
+    assume {:axiom} false; // todo
+  }
+}
+
